theories/IntersectionTypes/Util/sn_facts.v
@@ -1,0 +1,673 @@
+Require Import Undecidability.IntersectionTypes.CDV Undecidability.IntersectionTypes.Util.type_assignment_facts.
+Require Import Setoid Morphisms.
+Require Import List Lia.
+
+Import CDV (var, app, lam).
+
+Require Import ssreflect ssrbool ssrfun.
+
+Set Default Proof Using "Type".
+
+(*
+Lemma stepE M N : step M N ->
+  match M with
+  | app (app M1 M2) M3 => exists M', N = app M' M3 /\ step (app M1 M2) M'
+  | app (lam M1) M2 => N = (subst (scons M2 var) M1)
+  | lam (M1) => exists M', N = lam M' /\ step M1 M'
+  | _ => False
+  end.
+Proof. by case=> *; do ? eexists. Qed.
+*)
+
+#[local] Notation all P l := (fold_right and True (map P l)).
+
+Definition Arr (P Q : tm -> Prop) (M : tm) := forall N, P N -> Q (app M N).
+
+(*  forall N, (all (interp N) phi) -> interp (app M N) t *)
+
+Fixpoint interp (M : tm) (s : sty) : Prop :=
+  match s with
+  | atom a => sn M
+  | arr phi t => Arr (fun N => (all (interp N) phi)) (fun N => interp N t) M
+  end.
+
+Definition satis Gamma M t :=
+  (forall sigma, (forall i, Forall (interp (sigma i)) (nth i Gamma nil)) ->
+  interp (subst sigma M) t).
+
+Lemma Forall_all {X : Type} {P : X -> Prop} l : Forall P l <-> all P l.
+Proof.
+  elim: l. { done. }
+  move=> ?? IH. split.
+  - by move=> /Forall_cons_iff [? /IH].
+  - move=> [? ?]. constructor; first done. by apply /IH.
+Qed.
+
+(*
+Lemma head_redexE {M M'} : head_redex M M' ->
+  match M' with
+  | app (lam M1') M2' => M = subst (scons M2' var) M1'
+  | app M1' M2' => exists M1, M = app M1 M2' /\ head_redex M1 M1'
+  | _ => False
+  end.
+Proof.
+  elim. { done. }
+  move=> ? []; [done| |done].
+  move=> *. by eexists.
+Qed.
+
+Lemma head_redex_spec M N N' : step N N' -> head_redex M N -> M = N'.
+Proof.
+  elim /(measure_rect tm_size): M N N'.
+  move=> M IH N N' [].
+  - by move=> > /head_redexE.
+  - by move=> > ? /head_redexE.
+  - move=> > ? /head_redexE [?] [?] ?. subst.
+    congr app. apply: IH.
+    + move=> /=. lia.
+    + eassumption.
+    + eassumption.
+Qed.
+
+Lemma head_redex_interp M M' t : head_redex M M' -> interp M t -> interp M' t.
+Proof.
+  elim: t M M'.
+  { move=> ? M M' /= H HM. constructor=> N.
+    by move: H => /head_redex_spec /[apply] <-. }
+  move=> phi t IH M M' /= ? IH' N Hphi.
+  apply: IH. { apply: head_redex_app. eassumption. }
+  by apply: IH'.
+Qed.
+*)
+
+(* this will follow from saturation? *)
+Lemma interp_red M N t : interp (subst (scons N var) M) t -> interp (app (lam M) N) t.
+Proof.
+Admitted.
+
+(* no empty intersections *)
+Fixpoint positive (t : sty) :=
+  match t with
+  | atom _ => True
+  | arr phi t =>  phi <> nil /\ all positive phi /\ positive t
+  end.
+
+(* transforms a goal (A -> B) -> C into goals A and B -> C *)
+Lemma unnest : forall (A B C : Type), A -> (B -> C) -> (A -> B) -> C.
+Proof. auto. Qed.
+
+Inductive head_sn : tm -> Prop :=
+  | head_sn_var x : head_sn (var x)
+  | head_sn_app M N : head_sn M -> sn N -> head_sn (app M N).
+
+Inductive head_red : tm -> tm -> Prop :=
+  | head_red_lam M N : sn N -> head_red (subst (scons N var) M) (app (lam M) N)
+  | head_red_app M M' N : head_red M M' -> sn N -> head_red (app M N) (app M' N).
+
+Record Saturated (P : tm -> Prop) :=
+  { Saturated_sn : forall M, P M -> sn M;
+    Saturated_head_sn : forall M, head_sn M -> P M }.
+
+(* looks doable *)
+Lemma Saturated_interp t : positive t -> Saturated (fun M => interp M t).
+Proof.
+  elim /(measure_rect sty_size): t. case.
+  { move=> x IH _. constructor.
+    - done.
+    - move=> M /=. admit. (* easy *) }
+  move=> phi t IH /= [H1phi [H2phi Ht]]. constructor=> /=.
+  - move=> M. rewrite /Arr => HM.
+    have := HM (var 0).
+    apply: unnest. { admit. (* doabl? by IH *) }
+    have := IH t _ Ht.
+    apply: unnest. { rewrite /=. lia. }
+    move=> /Saturated_sn /[apply]. admit. (* doable *)
+  - move=> M HM N.
+    move: phi IH H1phi H2phi => [|s phi]; first done.
+    move=> IH _ /= [Hs Hphi] [].
+    have := IH s _ Hs.
+    apply: unnest. { rewrite /=. lia. }
+    move=> /Saturated_sn /[apply] ? H'phi.
+    have := IH t _ Ht.
+    apply: unnest. { rewrite /=. lia. }
+    move=> /Saturated_head_sn. apply.
+    by constructor.
+Admitted.
+
+(* this will follow from saturation *)
+Lemma interp_var x t : positive t -> interp (var x) t.
+Proof.
+  move=> /Saturated_interp /Saturated_head_sn. apply.
+  by constructor.
+Qed.
+
+(* this needs interp_var *)
+Lemma interp_sn M t : positive t -> interp M t -> sn M.
+Proof.
+  move=> /Saturated_interp /Saturated_sn. by apply.
+Qed.
+
+Lemma satisI Gamma M t : type_assignment Gamma M t -> satis Gamma M t.
+Proof.
+  elim: M Gamma t.
+  - move=> a > /type_assignmentE H.
+    by move=> sigma /(_ a) /Forall_forall /(_ _ H).
+  - move=> ? IH1 ? IH2 ?? /type_assignmentE [phi] [/IH1] {}IH1 Hphi.
+    move=> sigma Hsigma /=. apply: (IH1 sigma Hsigma).
+    apply /Forall_all. rewrite -/interp.
+    apply: Forall_impl Hphi => ? /IH2. by apply.
+  - move=> ? IH1 ? [?|phi t] /type_assignmentE; first done.
+    move=> /IH1 {}IH1 sigma HGamma /=.
+    move=> N Hphi. apply: interp_red. rewrite simpl_tm. apply: IH1 => - [|i].
+    + by apply /Forall_all.
+    + apply: Forall_impl (HGamma i) => ? /=.
+      by rewrite !simpl_tm.
+Qed.
+
+Lemma In_nth_In t x (Gamma : list ty) :
+  In t (nth x Gamma nil) ->
+  In (nth x Gamma nil) Gamma.
+Proof.
+  elim: Gamma x. { by case. }
+  by move=> > IH [|x] => [|/IH] ?; [left|right].
+Qed.
+
+Lemma normalization Gamma M t : 
+  Forall (Forall positive) Gamma -> positive t -> type_assignment Gamma M t -> sn M.
+Proof.
+  move=> HGamma Ht /satisI /(_ var). rewrite simpl_tm.
+  apply: unnest. 
+  { move=> i. apply /Forall_forall => ? /[dup] /In_nth_In.
+    move: HGamma => /Forall_forall /[apply].
+    move=> /Forall_forall /[apply].
+    by apply: interp_var. }
+  by apply: interp_sn.
+Qed.
+
+Print Assumptions normalization.
+
+(* OOOOOOOLD  *)
+
+Lemma Saturated_interp t : positive t -> Saturated (fun M => interp M t).
+Proof.
+  elim /(measure_rect sty_size): t. case.
+  { move=> x IH. constructor.
+    - done.
+    - move=> M /=. admit. (* easy *) }
+  move=> phi t IH /= H'. constructor=> /=.
+  - move=> M. rewrite /Arr => HM.
+    have := HM (var 0).
+    apply: unnest. { admit. (* doabl? by IH *) }
+
+
+Lemma head_sn_interp M t : head_sn M -> interp M t.
+Proof.
+  elim /(measure_rect sty_size): t M. case.
+  - move=> /= ? _. admit. (* easy *)
+  - move=> phi t IH /= M HM N Hphi. move=> ?. apply: (IH).
+    + move=> /=. lia.
+    +   rewrite /Arr.  
+
+Lemma head_sn_Arr (P Q : tm -> Prop) : (forall M, head_sn M -> P M) -> (forall M, head_sn M -> Q M) ->
+  forall M, head_sn M -> Arr P Q M.
+Proof.
+  move=> HP HQ ????. apply: HQ. constructor. elim.
+  - move=> x ? ?. apply: HQ.
+(* NO! need stratification 
+Lemma head_sn_interp M t : head_sn M -> interp M t.
+Proof.
+  elim /(measure_rect sty_size): t M. case.
+  - move=> /= ? _. admit. (* easy *)
+  - move=> phi t IH /= M HM N Hphi. apply: (IH).
+    + move=> /=. lia.
+    +   rewrite /Arr.  
+*)
+
+Lemma Saturated_interp t : Saturated (fun M => interp M t).
+Proof.
+  elim: t.
+  { constructor.
+    - move=> x /=. admit. (* easy *)
+    - move=> /=. admit. (* difficult *)
+    - move=> M N /=. (* WRONG *) admit. }
+  move=> phi t [???]. constructor.
+  - move=> x /=. rewrite /Arr.
+  constructor.
+
+(* OLD *)
+
+
+
+
+
+(* saturated set of lambda-terms 
+Definition sat (P : tm -> Prop) :=
+  (forall M, head_sn M -> P M) /\ (forall M M', head_redex M M' -> P M -> P M').
+*)
+
+(* saturated set of lambda-terms *)
+Definition sat (P : tm -> Prop) :=
+  (forall M, head_args sn M -> P M).
+
+Lemma sat_sn : sat sn.
+Proof.
+  move=> M H. have : head_form M.
+  split.
+Admitted.
+
+
+
+Lemma sat_Arr P Q : sat P -> sat Q -> sat (Arr P Q).
+Proof.
+  split.
+  - 
+  (*
+Lemma interp_sn M t : positive t -> interp M t -> sn M.
+Proof.
+  elim /(measure_rect sty_size) : t M.
+*)
+Lemma interp_hf M t : positive t -> head_sn M -> interp M t.
+Proof.
+  elim /(measure_rect sty_size) : t M.
+  case. { move=> a IH M /=. admit. (*doable  *) }
+  move=> [|s phi] t IH M /= []; first done.
+  move=> _ [[? ?] ?] HM N [H'N Hphi]. apply: (IH).
+  - move=> /=. lia.
+  - done.
+  - apply: head_sn_app; first done.
+
+
+
+
+
+
+
+
+
+Print Assumptions satisI.
+
+
+
+
+
+
+(*
+(*head form : x M1 .. Mn where x is free of bound*)
+Inductive normal_form : tm -> Prop :=
+  | normal_head : forall M, head_form M -> normal_form M
+  | normal_abs : forall M, normal_form M -> normal_form (lam M)
+  with head_form : tm -> Prop :=
+  | head_var : forall x, head_form (var x)
+  | head_app : forall M N, head_form M -> normal_form N -> head_form (app M N).
+
+Inductive sat (P : tm -> Prop) :=
+  (forall M, head_form M -> P M) /\ 
+*)
+
+Lemma asd M N t : step M N -> interp N t -> interp M t.
+Proof.
+  elim.
+  -  
+  - case: t.
+    + move=> /=.
+
+
+Definition pw_iff {X} p q := (forall x : X, p x <-> q x).
+Notation "p == q" := (pw_iff p q) (at level 70).
+
+#[local] Instance Equiv_pw_iff {X} : Equivalence (@pw_iff X).
+Proof. firstorder done. Qed.
+
+Lemma pw {X : Type} P Q :
+  (forall x : X, P x <-> Q x) ->
+  (forall x, P x) <-> (forall x, Q x).
+Proof. firstorder done. Qed.
+
+Ltac pw := repeat (apply pw; intros).
+
+(* * Strong Normalisation  *)
+
+(* ** Logical Relation  *)
+
+Definition active P :=
+  match P with
+  | lam _ => true
+  | _ => false
+  end.
+
+Definition tpred := tm -> Prop.
+
+Definition M (p : tpred) : tpred :=
+  fun P => forall xi, p (ren xi P).
+
+Inductive R (p : tpred) P : Prop :=
+| RI : (active P = true -> M p P) ->
+       (forall Q, step P Q -> R p Q) ->
+       R p P.
+
+#[local] Instance R_ext :
+  Proper (pw_iff ==> eq ==> iff) R.
+Proof.
+  intros p1 p2 Heq P ? ->. split; induction 1 as [P H H1 H2].
+  - econstructor. intros H3 xi. eapply Heq. now eapply H. eauto.
+  - econstructor. intros H3 xi. eapply Heq. now eapply H. eauto.
+Qed.
+
+Record model := mk_model
+  {
+    Var : tpred -> tpred ;
+    Arr : list tpred -> tpred -> tpred ;
+    Var_ext : Proper (pw_iff ==> pw_iff) Var ;
+    Arr_ext : Proper ((List.Forall2 pw_iff) ==> pw_iff ==> pw_iff) Arr ;
+  }.
+#[local] Existing Instances Var_ext Arr_ext.
+
+Section Evaluation.
+  Variable (M : model).
+
+  Fixpoint eval (ρ : nat -> tpred) (s : sty) : tpred :=
+    match s with
+    | atom a => Var M (ρ a)
+    | arr phi t => Arr M (map (eval ρ) phi) (eval ρ t)
+    end.
+
+  #[local] Instance eval_ext :
+    Proper (pointwise_relation _ pw_iff ==> eq ==> pw_iff) eval.
+  Proof.
+    intros ρ1 ρ2 Heq s ? <-. induction s in ρ1, ρ2, Heq |- *; cbn.
+    - now rewrite (Heq n).
+    - have ? : List.Forall2 pw_iff (map (eval ρ1) l) (map (eval ρ2) l).
+      admit. apply: Arr_ext. done. by apply: IHs.
+  Admitted.
+
+  (*
+  Lemma eval_ren ξ s ρ :
+    eval ρ (ren_poly_type ξ s) == eval (ξ >> ρ) s.
+  Proof.
+    induction s in ξ, ρ |- *; cbn.
+    - reflexivity.
+    - now rewrite IHs1, IHs2.
+    - eapply All_ext. intros d. rewrite IHs.
+      eapply eval_ext. now intros []. reflexivity.
+  Qed.
+
+  Lemma eval_weaken s ρ d :
+    eval (d .: ρ) (ren_poly_type shift s) == eval ρ s.
+  Proof. now rewrite eval_ren. Qed.
+*)
+
+  Definition lift : model.
+  Proof using M.
+    refine (mk_model id (Arr M) _ _).
+    abstract firstorder.
+  Defined.
+
+End Evaluation.
+
+(*
+Lemma eval_subst (M : model) σ s ρ :
+  eval M ρ (subst_poly_type σ s) == eval (lift M) (σ >> eval M ρ) s.
+Proof.
+  induction s in σ, ρ |- *; cbn.
+  - reflexivity.
+  - now rewrite IHs1, IHs2.
+  - eapply All_ext. intros d. rewrite IHs. asimpl.
+    eapply eval_ext; try reflexivity. intros []. reflexivity. eapply eval_weaken.
+Qed.
+
+
+Lemma eval_beta (M : model) s t ρ :
+  eval M ρ (subst_poly_type (t .: poly_var) s) == eval (lift M) (eval M ρ t .: ρ >> Var M) s.
+Proof.
+  rewrite eval_subst.
+  eapply eval_ext. now intros []. reflexivity.
+Qed.
+*)
+
+Definition D : model.
+Proof.
+  refine {| Var :=  id ;
+            Arr := fun ps q P => match P with lam P => forall Q, R p Q -> R q (subst_term poly_var (Q .: var) P) | _ => False end |}.
+  - abstract firstorder.
+  - abstract (intros p1 p2 Heq1 p1' p2' Heq2 []; cbn; try tauto; pw; now rewrite Heq1, Heq2).
+  - abstract (intros F1 F2 Heq []; cbn; try tauto; pw; now rewrite (Heq x)).
+Defined.
+
+(* Instance equiv_D : equiv D. *)
+
+Notation V s ρ := (eval D ρ s).
+Notation K s ρ := (M (V s ρ)).
+Notation E s ρ := (R (V s ρ)).
+
+(* ** Reducibility Candidates  *)
+
+Lemma R_sn p P :
+  R p P -> sn P.
+Proof.
+  induction 1. eauto using sn.
+Qed.
+
+Lemma R_step p P Q :
+  step P Q -> R p P -> R p Q.
+Proof.
+  intros ? []. eauto.
+Qed.
+
+Lemma R_var p n :
+  R p (var n).
+Proof.
+  econstructor. intros [=].
+  intros Q H. inversion H.
+Qed.
+
+Lemma R_ren ξ1 ξ2 p P :
+  R p P -> R p (ren_term ξ1 ξ2 P).
+Proof.
+  induction 1 as [P H H0 H1]. econstructor.
+  - intros HnP ξ'1 ξ'2. asimpl. eapply H. now destruct P.
+  - intros Q.  erewrite rinst_inst_term; try reflexivity.
+    intros (P' & H2 & <-) % step_subst_inv.
+    erewrite <- rinst_inst_term; try reflexivity. eauto.
+Qed.
+
+(* ** Logical Relation  *)
+
+Lemma K_var n ρ P :
+  K (poly_var n) ρ P = forall ξ1 ξ2, ρ n (ren_term ξ1 ξ2 P).
+Proof.
+  reflexivity.
+Qed.
+
+Lemma K_arr s t ρ u P :
+  K (poly_arr s t) ρ (abs u P) <->
+  forall ξ1 ξ2 Q, E s ρ Q -> E t ρ (subst_term (ξ1 >> poly_var) (Q .: ξ2 >> var) P).
+Proof.
+  unfold M. cbn. pw. asimpl. eapply R_ext. reflexivity.
+  now_asimpl.
+Qed.
+
+Lemma K_all s ρ P :
+  K (poly_abs s) ρ (ty_abs P) <->
+  forall ξ p t, E s (p .: ρ) (subst_term (t .: ξ >> poly_var) var P).
+Proof.
+  unfold M. split.
+  - intros H ξ p t. specialize (H ξ id p t). fold ren_term in H.
+    eapply R_ext. 3:eapply H. reflexivity. now_asimpl.
+  - intros H ξ1 ξ2 p t. specialize (H ξ1 p t).
+    pose proof (Hren := R_ren id ξ2 _ _ H). asimpl in Hren.
+    eapply R_ext. 3:eapply Hren. reflexivity. now_asimpl.
+Qed.
+
+Lemma V_weaken s ρ p :
+  V (ren_poly_type shift s) (p .: ρ) == V s ρ.
+Proof.
+  now rewrite eval_weaken.
+Qed.
+
+Lemma K_weaken s ρ p :
+  K (ren_poly_type shift s) (p .: ρ) == K s ρ.
+Proof.
+  intros P. pw. eapply V_weaken.
+Qed.
+
+Lemma E_weaken s ρ p :
+  E (ren_poly_type shift s) (p .: ρ) == E s ρ.
+Proof.
+  intros P. eapply R_ext. eapply V_weaken. reflexivity.
+Qed.
+
+Lemma V_beta s t ρ :
+  V (subst_poly_type (t .: poly_var) s) ρ == V s (V t ρ .: ρ).
+Proof.
+  now rewrite eval_beta. 
+Qed.
+
+Lemma E_beta  s t ρ :
+  E (subst_poly_type (t .: poly_var) s) ρ == E s (V t ρ .: ρ).
+Proof.
+  intros P. now rewrite eval_beta. 
+Qed.
+
+(* ** Logical relation on contexts  *)
+
+Definition C (Γ : nat -> poly_type) (ρ : nat -> tpred) : (nat -> term) -> Prop :=
+  fun σ => forall n, E (Γ n) ρ (σ n).
+
+Lemma C_ext :
+  Proper (pointwise_relation _ eq ==> eq ==> eq ==> iff) C.
+Proof.
+  split; repeat intros ?; subst. now rewrite <- H. now rewrite H.
+Qed.
+
+Lemma C_scons s Γ ρ σ P :
+  E s ρ P -> C Γ ρ σ -> C (s .: Γ) ρ (P .: σ).
+Proof.
+  intros HE HC. hnf. intros []. eassumption. eapply HC.
+Qed.
+
+Lemma C_rename Γ ρ σ ξ1 ξ2 :
+  C Γ ρ σ -> C Γ ρ (σ >> ren_term ξ1 ξ2).
+Proof.
+  intros H ?. eapply R_ren, H.
+Qed.
+
+Lemma C_up s Γ ρ σ :
+  C Γ ρ σ -> C (s .: Γ) ρ (up_term_term σ).
+Proof.
+  intros H. eapply C_scons. eapply R_var. now eapply C_rename.
+Qed.
+
+(* ** Fundamental theorem & Strong Normalisation  *)
+Lemma E2_ind s t ρ1 ρ2 p :
+  (forall P Q, E s ρ1 P -> E t ρ2 Q -> (forall P', step P P' -> p P' Q) -> (forall Q', step Q Q' -> p P Q') -> p P Q) ->
+  forall P Q, E s ρ1 P -> E t ρ2 Q -> p P Q.
+Proof.
+  intros H P Q. 
+  induction 1 in Q |- *. induction 1. 
+  eapply H; eauto using R.
+Qed.
+
+Lemma E_app s t P Q ρ :
+  E (poly_arr s t) ρ P -> E s ρ Q -> E t ρ (app P Q).
+Proof.
+  revert P Q. eapply E2_ind.
+  intros P Q nP nQ IHP IHQ. econstructor.
+  inversion 1. intros R Hst. inv Hst; eauto.
+  destruct nP. rewrite K_arr in H; eauto.
+Qed.
+
+Lemma E_lam s t s' ρ P :
+  sn P ->
+  (forall ξ1 ξ2 Q, E s ρ Q -> E t ρ (subst_term (ξ1 >> poly_var) (Q .: ξ2 >> var) P)) ->
+  E (poly_arr s t) ρ (abs s' P).
+Proof.
+    induction 1 as [P _ IH]. intros H.
+    econstructor.
+    - intros _. rewrite K_arr. eauto.
+    - intros Q Hst. inv Hst. eapply IH; eauto.
+      intros. eapply R_step; eauto using step_subst.
+Qed.
+
+Lemma E_tapp s t ρ P r :
+  E (poly_abs s) ρ P -> E (subst_poly_type (t .: poly_var) s) ρ (ty_app P r).
+Proof.
+  induction 1 as [P H IH H2]. eapply E_beta.
+  econstructor. inversion 1. intros Q Hst. inv Hst.
+  - specialize (H eq_refl). rewrite K_all in H. eauto.
+  - eapply H2 in H4. now eapply E_beta in H4.
+Qed.
+
+Lemma E_tlam s ρ P :
+  sn P ->
+  (forall ξ p t, E s (p .: ρ) (subst_term (t .: ξ >> poly_var) var P)) ->
+  E (poly_abs s) ρ (ty_abs P).
+Proof.
+  induction 1 as [P _ IH]. intros H. econstructor.
+  - rewrite K_all. intros _. eapply H.
+  - intros Q Hst. inv Hst. eapply IH. eauto.
+    intros ξ p t.
+    eapply R_step; eauto using step_subst.
+Qed.
+
+Lemma fundamental {Γ s P} :
+  typing Γ P s ->
+  forall σ τ ρ, 
+  C (fun n => match List.nth_error Γ n with Some x => x | _ => poly_abs (poly_var 0) end) ρ τ -> 
+  E s ρ (subst_term σ τ P).
+Proof.
+  induction 1 as [Γ n s H | | Γ | | ]; intros σ τ ρ HC.
+  - specialize (HC n). cbn in HC. rewrite H in HC. eapply HC.
+  - cbn. eapply E_app; eauto.
+  -  eapply E_lam; fold subst_term.
+     + eapply R_sn. eapply IHtyping.
+       eapply C_ext. 4:{ eapply C_up, HC. }
+       all: try reflexivity.
+       now intros []. 
+     + intros ξ1 ξ2 Q HQ.
+       match goal with [ |- E _ _ ?R] => 
+                       replace R with (subst_term (σ >> ren_poly_type ξ1) (Q .: τ >> ren_term ξ1 ξ2) P)
+       end.
+       * eapply IHtyping. eapply C_ext.
+         4:{ eapply C_scons. eauto. eapply C_rename, HC. }
+         all: try reflexivity.
+         intros []; cbn; try reflexivity.
+       * asimpl. eapply ext_term. intros. asimpl.
+         -- erewrite rinst_inst_poly_type; reflexivity.
+         -- intros []. reflexivity. asimpl.
+            erewrite rinst_inst_term; try reflexivity. now asimpl.
+  - cbn. eapply E_tapp; eauto.
+  - cbn. eapply E_tlam.
+    + specialize (IHtyping (up_poly_type_poly_type σ) (τ >> ren_term shift id) ((fun _ => False) .: ρ)).
+      eapply R_sn. refine (IHtyping _).
+      intros n.
+      rewrite List.nth_error_map.
+      destruct List.nth_error eqn:Eq.
+      * cbn. asimpl. eapply E_weaken.
+        specialize (HC n). cbn in HC. rewrite Eq in HC.
+        eapply R_ren, HC.
+      * unfold ssrfun.Option.map, ssrfun.Option.bind, ssrfun.Option.apply.
+        eapply R_ren. specialize (HC n). cbn in HC.
+        rewrite Eq in HC. eapply HC.
+    + intros ξ p t. asimpl. eapply IHtyping.
+      intros n. asimpl. eapply R_ext. 2:reflexivity.
+      2:{ eapply E_weaken.
+          erewrite <- rinst_inst_term; try reflexivity.
+          eapply R_ren. eapply HC. }
+      * f_equal. rewrite List.nth_error_map.
+        now destruct List.nth_error eqn:Eq.
+Qed.
+
+Lemma SN {Gamma P t} : typing Gamma P t -> sn P.
+Proof.
+  intros Htp. pose proof (fundamental Htp poly_var var (fun _ _ => False)).
+  asimpl in H.
+  eapply R_sn, H.
+  intros n. eapply R_var.
+Qed.
+
+Lemma typing_normal_form {Gamma P t} : typing Gamma P t -> exists Q, normal_form Q /\ typing Gamma Q t.
+Proof.
+  intros H.
+  destruct (sn_normal _ _ _ H (SN H)) as (Q & H1 & H2).
+  exists Q. split. eassumption. eapply preservation_star; eauto.
+Qed.
